证明：
$$
\sin (\alpha +\beta )= \sin \alpha \cos \beta +\cos \alpha \sin \beta 
$$
![](https://cdn.jsdelivr.net/gh/breezyfrost/image-host/202408290922555.png)

单位圆中：
$$
\begin{alignat}{2}  
\sin (\alpha +\beta ) &= CE + ED \\
&= \frac{CF}{\cos \alpha} + ED \\
&= \frac{\sin \beta}{\cos \alpha } + ED \\
&= \frac{\sin \beta}{\cos \alpha }  + (AF -EF)\sin \alpha  \\
&= \frac{\sin \beta}{\cos \alpha }  + (\cos \beta - EF)\sin \alpha \\
&= \frac{\sin \beta}{\cos \alpha }  + (\cos \beta - CE \sin \alpha )\sin \alpha \\
&= \frac{\sin \beta}{\cos \alpha }  + (\cos \beta - \frac{\sin \beta}{\cos \alpha } \sin \alpha )\sin \alpha \\
&= \frac{\sin \beta}{\cos \alpha } + \sin \alpha \cos \beta - \frac{\sin \beta \sin^2 \alpha}{\cos \alpha }  \\
&= \sin \alpha \cos \beta + \frac{\sin \beta (1-\sin^2 \alpha)}{\cos \alpha }  \\
&= \sin \alpha \cos \beta + \frac{\sin \beta \cos^2 \alpha}{\cos \alpha }  \\
&= \sin \alpha \cos \beta + \sin \beta \cos \alpha \\
\end{alignat}
$$
